code/Yazi.Adler32.fsti
@@ -1,5 +1,6 @@
 module Yazi.Adler32
 module B = LowStar.Buffer
+module CB = LowStar.ConstBuffer
 module Cast = FStar.Int.Cast
 module Spec = Spec.Adler32
 module U32 = FStar.UInt32
@@ -16,13 +17,14 @@ val adler32:
     #m: Ghost.erased nat
   -> data: Ghost.erased (Spec.input m)
   -> adler: U32.t
-  -> buf: B.buffer U8.t
+  -> buf: CB.const_buffer U8.t
   -> len: U32.t
   -> ST.Stack U32.t
-  (requires fun h -> B.live h buf /\ B.length buf == U32.v len /\ Spec.adler32_matched data adler)
+  (requires fun h ->
+    CB.live h buf /\ CB.length buf == U32.v len /\ Spec.adler32_matched data adler)
   (ensures fun h0 res h1 ->
     B.(modifies loc_none h0 h1) /\
-    Spec.adler32_matched #(m + U32.v len) (Seq.append data (B.as_seq h1 buf)) res)
+    Spec.adler32_matched #(m + U32.v len) (Seq.append data (CB.as_seq h1 buf)) res)
 
 val adler32_combine64:
     #m1: Ghost.erased nat
