code/Yazi.CRC32.fst
@@ -1,6 +1,7 @@
 module Yazi.CRC32
 
 module B = LowStar.Buffer
+module CB = LowStar.ConstBuffer
 module Spec = Spec.CRC32
 module ST = FStar.HyperStack.ST
 module U32 = FStar.UInt32
@@ -10,14 +11,14 @@ module U8 = FStar.UInt8
 assume val crc32:
     data: Ghost.erased (Seq.seq U8.t)
   -> crc: U32.t
-  -> buf: B.buffer U8.t
+  -> buf: CB.const_buffer U8.t
   -> len: U32.t
   -> ST.Stack U32.t
   (requires fun h ->
-    B.live h buf /\ B.length buf == U32.v len /\
+    CB.live h buf /\ CB.length buf == U32.v len /\
     Spec.crc32_matched (Seq.length data) data crc true)
   (ensures fun h0 res h1 ->
     B.(modifies loc_none h0 h1) /\
     Spec.crc32_matched
       (Seq.length data + U32.v len)
-      (Seq.append data (B.as_seq h1 buf)) res true)
+      (Seq.append data (CB.as_seq h1 buf)) res true)
